one case of adequacy

KLR/Semantics/Logic.lean
@@ -11,14 +11,16 @@ import Iris.Algebra.OFE
 import Iris.Algebra.UPred
 import Iris.Instances.UPred
 import Iris.Instances.heProp
-import Iris.BI.BI
+import Iris.BI
+import Iris.ProofMode
+import Iris.BI.DerivedLaws
 
 -- The logic: I can reuse UPred with a fixed ghost state (first-order)
 -- I'll want the fixpoint combinator to define the wp
 -- Need to port some more of the upred rules most likely
 
 section weakestpre
-open Iris.BI.BIBase KLR.Core
+open Iris.BI.BIBase KLR.Core Iris NML
 
 variable {DataT : Type _}
 
@@ -27,55 +29,75 @@ abbrev state := (NML.NMLSemantics DataT).State
 abbrev val := (NML.NMLSemantics DataT).Val
 abbrev step := (NML.NMLSemantics DataT).Step
 abbrev to_val := (NML.NMLSemantics DataT).toVal
+abbrev StepN := (NML.NMLSemantics DataT).StepN
 
 abbrev PROP : Type _ := heProp PNat ProdIndex (UCell UInt8 DataT) ProdChipMemory
 
 -- The state interpretation, ie the global version of the program state.
-def state_interp (l r : @state DataT) : @PROP DataT :=
-  heProp_auth _ _ _ _ (.mk l.memory r.memory)
-  -- Strong relational invariant goes here?
+def state_interp (left right : @state DataT) : @PROP DataT :=
+  heProp_auth _ _ _ _ (.mk left.memory right.memory)
 
 def wp_F (wp : @prog DataT → @prog DataT → (@val DataT → @val DataT → @PROP DataT) → @PROP DataT)
          (p1 p2 : @prog DataT)
          (Φf : @val DataT → @val DataT → @PROP DataT) : @PROP DataT :=
   -- For any pair of states that satisfy the state interpretation...
-  «forall» fun sl : @state DataT =>
-  «forall» fun sr : @state DataT =>
-    iprop(state_interp sl sr -∗
+  iprop(∀ sl, ∀ sr, state_interp sl sr -∗
       -- Either, that configuration is a value, and the postcondition holds,
-      (|==>
-        «exists» fun vl : @val DataT =>
-        «exists» fun vr : @val DataT =>
-        iprop(⌜to_val p1 = some vl⌝ ∗ ⌜to_val p2 = some vr⌝ ∗ Φf vl vr)) ∨
-      -- Or, for any two configurations that we can step into, in some number of steps,
-      ( «forall» fun cl' : @prog DataT × @state DataT =>
-        «forall» fun cr' : @prog DataT × @state DataT =>
-        «exists» fun nl : Nat =>
-        «exists» fun nr : Nat =>
-        iprop(
-          ⌜(NML.NMLSemantics DataT).StepN nl.succ (p1, sl) cl' ∧
-            (NML.NMLSemantics DataT).StepN nr.succ (p2, sr) cr'⌝ -∗
+      (|==> ∃ vl, ∃ vr, ⌜to_val p1 = some vl⌝ ∗ ⌜to_val p2 = some vr⌝ ∗ Φf vl vr) ∨
+      -- Or, they're not values, and for any two configurations that we can step into, in some number of steps,
+      ( ⌜to_val p1 = none ∨ to_val p2 = none⌝ ∗
+        ∀ cl', ∀ cr', ∀ nl, ∀ nr,
+          ⌜StepN (Nat.succ nl) (p1, sl) cl' ∧ StepN (Nat.succ nr) (p2, sr) cr'⌝ -∗
             -- We can reobtain the state interp for the new state, and also
             -- prove the weakest precondition.
-            ▷ |==> (state_interp cl'.2 cr'.2 ∗ wp cl'.1 cr'.1 Φf))))
+            ▷ |==> (state_interp cl'.2 cr'.2 ∗ wp cl'.1 cr'.1 Φf)))
 
-instance : Iris.OFE.Contractive (α := @prog DataT → @prog DataT → (@val DataT → @val DataT → @PROP DataT) → @PROP DataT) wp_F := by
+instance wp_contractive : Iris.OFE.Contractive (α := @prog DataT → @prog DataT → (@val DataT → @val DataT → @PROP DataT) → @PROP DataT) wp_F := by
   sorry
 
 /-- Definition of the weakest precondition -/
 def wp (p1 p2 : @prog DataT) (Φf : @val DataT → @val DataT → @PROP DataT) : @PROP DataT :=
   (Iris.fixpoint wp_F) p1 p2 Φf
 
+theorem wp_unfold {p1 p2 : @prog DataT} {Φf : @val DataT → @val DataT → @PROP DataT} :
+    wp p1 p2 Φf ≡
+    iprop(∀ sl, ∀ sr, state_interp sl sr -∗
+      (|==> ∃ vl, ∃ vr, ⌜to_val p1 = some vl⌝ ∗ ⌜to_val p2 = some vr⌝ ∗ Φf vl vr) ∨
+      ( ⌜to_val p1 = none ∨ to_val p2 = none⌝ ∗
+        ∀ cl', ∀ cr', ∀ nl, ∀ nr,
+          ⌜StepN (Nat.succ nl) (p1, sl) cl' ∧ StepN (Nat.succ nr) (p2, sr) cr'⌝ -∗
+            ▷ |==> (state_interp cl'.2 cr'.2 ∗ wp cl'.1 cr'.1 Φf))) := by
+  apply fixpoint_unfold (f := ⟨wp_F, OFE.ne_of_contractive wp_F⟩)
+
 end weakestpre
 
 /-- If the two terms are values, then we at the very least get a relationship between their values. -/
-theorem wp_value_value_fupd {pl pr : @prog DataT} {Φf : @val DataT → @val DataT → Prop}
+theorem wp_value_value_fupd {pl pr : @prog DataT} {sl sr : @state DataT} {Φf : @val DataT → @val DataT → Prop}
     (Hpl : (NML.NMLSemantics DataT).IsValue pl) (Hpr : (NML.NMLSemantics DataT).IsValue pr) :
-    wp pl pr (fun vl vr => iprop(⌜(Φf vl vr : Prop)⌝)) ⊢
-      |==> ⌜∃ (vl vr : @val DataT), to_val pl = some vl ∧ to_val pr = some vr ∧ Φf vl vr⌝ := by
-  -- I need internal eq to actually do this unfolding.
-  unfold wp
-  sorry
+    state_interp sl sr ∗ wp pl pr (fun vl vr => iprop(⌜(Φf vl vr : Prop)⌝)) ⊢
+            |==> ⌜∃ (vl vr : @val DataT), to_val pl = some vl ∧ to_val pr = some vr ∧ Φf vl vr⌝ := by
+  apply Iris.BI.entails_trans.trans (Iris.BI.equiv_iff.mp (Iris.BI.sep_ne.eqv .rfl wp_unfold)).mp
+  istart
+  iintro ⟨Hs, Hwp⟩
+  ispecialize Hwp Hs
+  istop
+  apply Iris.BI.entails_trans.trans Iris.BI.emp_sep.1
+  istart
+  iintro (Hv|⟨⌜Hk⌝, _⟩)
+  · istop
+    apply Iris.BIUpdate.mono _
+    istart
+    iintro ⟨vl, vr, ⌜Hvl⌝, ⌜Hvr⌝⟩
+    ipure_intro
+    exists vl
+    exists vr
+  · exfalso
+    unfold to_val at *
+    unfold SmallStep.IsValue at *
+    rcases Hk with (Hk | Hk)
+    · rw [Hk] at Hpl; cases Hpl
+    · rw [Hk] at Hpr; cases Hpr
+
 
 /-- Definition for Hoare Triple -/
 def triple (pre : @PROP DataT) (p1 p2 : @prog DataT) post :=
